# 67. Add Binary

[link](https://leetcode.com/problems/add-binary/description/)

Tags: String

Difficulty: Easy

## Description

Given two binary strings, return their sum (also a binary string).

For example,
a = `"11"`
b = `"1"`
Return `"100"`.

## Solutions

### 1. good short solution

```c++
class Solution
{
public:
    string addBinary(string a, string b)
    {
        string s = "";
        
        int c = 0, i = a.size() - 1, j = b.size() - 1;
        while(i >= 0 || j >= 0 || c == 1)
        {
            c += i >= 0 ? a[i --] - '0' : 0;
            c += j >= 0 ? b[j --] - '0' : 0;
            s = char(c % 2 + '0') + s;
            c /= 2;
        }
        
        return s;
    }
};
```

### 2. use bitwise xor

```c++
string addBinary(string a, string b) 
{
    string result = "";
    int apos = a.size() - 1;
    int bpos = b.size() - 1;
    int adigit, bdigit, carry = 0;
    
    while (apos >= 0 || bpos >= 0 || carry == 1)
    {
        adigit = bdigit = 0;
        
        if (apos >= 0) adigit = a[apos--] == '1';
        if (bpos >= 0) bdigit = b[bpos--] == '1';
        
        // Another way: the digit is 1 if adigit + bdigit + carry == 1 or == 3, but I noticed that
        // XOR is more concise:
        result = static_cast<char>(adigit ^ bdigit ^ carry + '0') + result; 
        carry = adigit + bdigit + carry >= 2;
    }
    
    return result;
}
```

### 3. my solution

```c++
class Solution {
public:
    string addBinary(string a, string b) {
        if (a.empty()) return b;
        if (b.empty()) return a;
        
        int len1 = a.length();
        int len2 = b.length();
        // make sure string a is the longer string
        if (len1 < len2) {
            a.swap(b);
            int temp = len1;
            len1 = len2;
            len2 = temp;
        }
        string sum(len1, '0');
        int carry = 0;
        int i;
        for (i = 0; i < len2; i++) {
            sum[len1-i-1] = (a[len1-i-1] -'0' + b[len2-i-1] - '0' + carry) % 2 + '0';   // remember to +'0'!!!
            carry = (a[len1-i-1] -'0' + b[len2-i-1] - '0' + carry) / 2;
        }
        for ( ; i < len1; i++) {
            sum[len1-i-1] = (a[len1-i-1] - '0' + carry) % 2 + '0';
            carry = (a[len1-i-1] - '0' + carry) / 2;
        }
        if (carry == 1)
            sum.insert(0, "1");
        
        return sum;
    }
};
```

